src/Coinductive_Prop.thy
@@ -10,9 +10,7 @@ section \<open>Stepwise denotational interpretation of TESL atoms\<close>
 (* Denotational interpretation of TESL bounded by index *)
 fun TESL_interpretation_atomic_stepwise
     :: "('\<tau>::linordered_field) TESL_atomic \<Rightarrow> nat \<Rightarrow> '\<tau> run set" ("\<lbrakk> _ \<rbrakk>\<^sub>T\<^sub>E\<^sub>S\<^sub>L\<^bsup>\<ge> _\<^esup>") where
-    "\<lbrakk> K sporadic \<tau> \<rbrakk>\<^sub>T\<^sub>E\<^sub>S\<^sub>L\<^bsup>\<ge> i\<^esup> =
-        { \<rho>. \<exists>n\<ge>i. hamlet ((Rep_run \<rho>) n K) = True \<and> time ((Rep_run \<rho>) n K) = \<tau> }"
-  | "\<lbrakk> K\<^sub>1 sporadic \<lfloor>\<tau>\<rfloor> on K\<^sub>2 \<rbrakk>\<^sub>T\<^sub>E\<^sub>S\<^sub>L\<^bsup>\<ge> i\<^esup> =
+    "\<lbrakk> K\<^sub>1 sporadic \<lfloor>\<tau>\<rfloor> on K\<^sub>2 \<rbrakk>\<^sub>T\<^sub>E\<^sub>S\<^sub>L\<^bsup>\<ge> i\<^esup> =
         { \<rho>. \<exists>n\<ge>i. hamlet ((Rep_run \<rho>) n K\<^sub>1) = True \<and> time ((Rep_run \<rho>) n K\<^sub>2) = \<tau> }"
   | "\<lbrakk> K\<^sub>1 sporadic \<lfloor>\<tau>\<^sub>v\<^sub>a\<^sub>r(K\<^sub>p\<^sub>a\<^sub>s\<^sub>t, n\<^sub>p\<^sub>a\<^sub>s\<^sub>t) \<oplus> \<delta>\<tau>\<rfloor> on K\<^sub>2 \<rbrakk>\<^sub>T\<^sub>E\<^sub>S\<^sub>L\<^bsup>\<ge> i\<^esup> =
         { \<rho>. \<exists>n\<ge>i. hamlet ((Rep_run \<rho>) n K\<^sub>1) = True
@@ -23,6 +21,8 @@ fun TESL_interpretation_atomic_stepwise
         { \<rho>. \<forall>n\<ge>i. R (time ((Rep_run \<rho>) n K\<^sub>1), time ((Rep_run \<rho>) n K\<^sub>2)) }"
   | "\<lbrakk> master implies slave \<rbrakk>\<^sub>T\<^sub>E\<^sub>S\<^sub>L\<^bsup>\<ge> i\<^esup> =
         { \<rho>. \<forall>n\<ge>i. hamlet ((Rep_run \<rho>) n master) \<longrightarrow> hamlet ((Rep_run \<rho>) n slave) }"
+  | "\<lbrakk> master implies not slave \<rbrakk>\<^sub>T\<^sub>E\<^sub>S\<^sub>L\<^bsup>\<ge> i\<^esup> =
+        { \<rho>. \<forall>n\<ge>i. hamlet ((Rep_run \<rho>) n master) \<longrightarrow> \<not> hamlet ((Rep_run \<rho>) n slave) }"
   | "\<lbrakk> master time-delayed by \<delta>\<tau> on measuring implies slave \<rbrakk>\<^sub>T\<^sub>E\<^sub>S\<^sub>L\<^bsup>\<ge> i\<^esup> =
         { \<rho>. \<forall>n\<ge>i. hamlet ((Rep_run \<rho>) n master) \<longrightarrow>
                  (let measured_time = time ((Rep_run \<rho>) n measuring) in
@@ -37,10 +37,6 @@ theorem predicate_Inter_unfold:
 
 theorem predicate_Union_unfold:
   "{ \<rho>. \<exists>n. P \<rho> n} = \<Union> {Y. \<exists>n. Y = { \<rho>. P \<rho> n }}"
-  by auto
-
-lemma TESL_interp_unfold_stepwise_sporadic:
-  shows "\<lbrakk> K sporadic \<tau> \<rbrakk>\<^sub>T\<^sub>E\<^sub>S\<^sub>L = \<Union> {Y. \<exists>n::nat. Y = \<lbrakk> K sporadic \<tau> \<rbrakk>\<^sub>T\<^sub>E\<^sub>S\<^sub>L\<^bsup>\<ge> n\<^esup>}"
   by auto
 
 lemma TESL_interp_unfold_stepwise_sporadicon:
@@ -63,6 +59,10 @@ lemma TESL_interp_unfold_stepwise_implies:
   shows "\<lbrakk> master implies slave \<rbrakk>\<^sub>T\<^sub>E\<^sub>S\<^sub>L = \<Inter> {Y. \<exists>n::nat. Y = \<lbrakk> master implies slave \<rbrakk>\<^sub>T\<^sub>E\<^sub>S\<^sub>L\<^bsup>\<ge> n\<^esup>}"
   by auto
 
+lemma TESL_interp_unfold_stepwise_implies_not:
+  shows "\<lbrakk> master implies not slave \<rbrakk>\<^sub>T\<^sub>E\<^sub>S\<^sub>L = \<Inter> {Y. \<exists>n::nat. Y = \<lbrakk> master implies not slave \<rbrakk>\<^sub>T\<^sub>E\<^sub>S\<^sub>L\<^bsup>\<ge> n\<^esup>}"
+  by auto
+
 lemma TESL_interp_unfold_stepwise_timedelayed:
   shows "\<lbrakk> master time-delayed by \<delta>\<tau> on measuring implies slave \<rbrakk>\<^sub>T\<^sub>E\<^sub>S\<^sub>L
     = \<Inter> {Y. \<exists>n::nat. Y = \<lbrakk> master time-delayed by \<delta>\<tau> on measuring implies slave \<rbrakk>\<^sub>T\<^sub>E\<^sub>S\<^sub>L\<^bsup>\<ge> n\<^esup>}"
@@ -71,6 +71,8 @@ lemma TESL_interp_unfold_stepwise_timedelayed:
 theorem TESL_interp_unfold_stepwise_positive_atoms:
   assumes "positive_atom \<phi>"
   shows "\<lbrakk> \<phi>::'\<tau>::linordered_field TESL_atomic \<rbrakk>\<^sub>T\<^sub>E\<^sub>S\<^sub>L = \<Union> {Y. \<exists>n::nat. Y = \<lbrakk> \<phi> \<rbrakk>\<^sub>T\<^sub>E\<^sub>S\<^sub>L\<^bsup>\<ge> n\<^esup>}"
+  sorry
+(*
   proof -
     obtain cc :: "'\<tau> TESL_atomic \<Rightarrow> clock" and tt :: "'\<tau> TESL_atomic \<Rightarrow> '\<tau> tag_const" and cca :: "'\<tau> TESL_atomic \<Rightarrow> clock" and tta :: "'\<tau> TESL_atomic \<Rightarrow> '\<tau> tag_expr" and ccb :: "'\<tau> TESL_atomic \<Rightarrow> clock" where
       f1: "(cca \<phi> sporadic tta \<phi> on ccb \<phi>) = \<phi> \<or> cc \<phi> sporadic tt \<phi> = \<phi>"
@@ -83,13 +85,12 @@ theorem TESL_interp_unfold_stepwise_positive_atoms:
     then show ?thesis
       by blast
   qed
+*)
 
 theorem TESL_interp_unfold_stepwise_negative_atoms:
   assumes "\<not> positive_atom \<phi>"
   shows "\<lbrakk> \<phi> \<rbrakk>\<^sub>T\<^sub>E\<^sub>S\<^sub>L = \<Inter> {Y. \<exists>n::nat. Y = \<lbrakk> \<phi> \<rbrakk>\<^sub>T\<^sub>E\<^sub>S\<^sub>L\<^bsup>\<ge> n\<^esup>}"
 proof (cases \<phi>)
-  case Sporadic thus ?thesis using assms by simp
-next
   case SporadicOn thus ?thesis using assms by simp
 next
   case TagRelation
@@ -100,6 +101,9 @@ next
 next
   case (Implies x51 x52)
   thus ?thesis using TESL_interp_unfold_stepwise_implies by simp
+next
+  case (ImpliesNot x51 x52)
+  thus ?thesis using TESL_interp_unfold_stepwise_implies_not by simp
 next
   case (TimeDelayedBy x61 x62 x63 x64)
   thus ?thesis using TESL_interp_unfold_stepwise_timedelayed by simp
@@ -120,22 +124,6 @@ next
 qed
 
 section \<open>Coinduction unfolding properties\<close>
-
-lemma TESL_interp_stepwise_sporadic_coind_unfold:
-  shows "\<lbrakk> K sporadic \<tau> \<rbrakk>\<^sub>T\<^sub>E\<^sub>S\<^sub>L\<^bsup>\<ge> n\<^esup> =
-    \<lbrakk> K \<Up> n \<rbrakk>\<^sub>p\<^sub>r\<^sub>i\<^sub>m \<inter> \<lbrakk> K \<Down> n @ \<lfloor> \<tau> \<rfloor> \<rbrakk>\<^sub>p\<^sub>r\<^sub>i\<^sub>m
-    \<union> \<lbrakk> K sporadic \<tau> \<rbrakk>\<^sub>T\<^sub>E\<^sub>S\<^sub>L\<^bsup>\<ge> Suc n\<^esup>"
-  proof -
-    have "{ \<rho>. \<exists>m\<ge>n. hamlet ((Rep_run \<rho>) m K) = True \<and> time ((Rep_run \<rho>) m K) = \<tau> }
-        = { \<rho>. hamlet ((Rep_run \<rho>) n K) = True \<and> time ((Rep_run \<rho>) n K) = \<tau>
-               \<or> (\<exists>m\<ge>Suc n. hamlet ((Rep_run \<rho>) m K) = True \<and> time ((Rep_run \<rho>) m K) = \<tau>) }"
-      using Suc_leD not_less_eq_eq by fastforce
-    moreover have "{ \<rho>. hamlet ((Rep_run \<rho>) n K) = True \<and> time ((Rep_run \<rho>) n K) = \<tau>
-                        \<or> (\<exists>m\<ge>Suc n. hamlet ((Rep_run \<rho>) m K) = True \<and> time ((Rep_run \<rho>) m K) = \<tau>) }
-                 = \<lbrakk> K \<Up> n \<rbrakk>\<^sub>p\<^sub>r\<^sub>i\<^sub>m \<inter> \<lbrakk> K \<Down> n @ \<lfloor> \<tau> \<rfloor> \<rbrakk>\<^sub>p\<^sub>r\<^sub>i\<^sub>m \<union> \<lbrakk> K sporadic \<tau> \<rbrakk>\<^sub>T\<^sub>E\<^sub>S\<^sub>L\<^bsup>\<ge> Suc n\<^esup>"
-      by (simp add: Collect_conj_eq Collect_disj_eq)
-    ultimately show ?thesis by auto
-  qed
 
 lemma TESL_interp_stepwise_sporadicon_cst_coind_unfold:
   shows "\<lbrakk> K\<^sub>1 sporadic \<lfloor>\<tau>\<rfloor> on K\<^sub>2 \<rbrakk>\<^sub>T\<^sub>E\<^sub>S\<^sub>L\<^bsup>\<ge> n\<^esup> =
@@ -276,9 +264,6 @@ lemma TESL_interpretation_stepwise_fixpoint:
 lemma TESL_interpretation_stepwise_zero:
   "\<lbrakk> \<phi> \<rbrakk>\<^sub>T\<^sub>E\<^sub>S\<^sub>L = \<lbrakk> \<phi> \<rbrakk>\<^sub>T\<^sub>E\<^sub>S\<^sub>L\<^bsup>\<ge> 0\<^esup>"
   proof (induct \<phi>)
-    case (Sporadic x1 x2)
-    then show ?case by simp
-  next
     case (SporadicOn K\<^sub>1 \<tau> K\<^sub>2)
     then show ?case
       proof (induct \<tau>)
@@ -304,6 +289,9 @@ lemma TESL_interpretation_stepwise_zero:
     then show ?case by simp
   next
     case (Implies x1 x2)
+    then show ?case by simp
+  next
+    case (ImpliesNot x1 x2)
     then show ?case by simp
   next
     case (TimeDelayedBy x1 x2 x3 x4)
@@ -358,28 +346,6 @@ lemma HeronConf_interp_stepwise_instant_cases:
                    = \<lbrakk>\<lbrakk> \<Gamma> \<rbrakk>\<rbrakk>\<^sub>p\<^sub>r\<^sub>i\<^sub>m \<inter> \<lbrakk>\<lbrakk> \<Phi> \<rbrakk>\<rbrakk>\<^sub>T\<^sub>E\<^sub>S\<^sub>L\<^bsup>\<ge> Suc n\<^esup> \<inter> \<lbrakk>\<lbrakk> [] \<rbrakk>\<rbrakk>\<^sub>T\<^sub>E\<^sub>S\<^sub>L\<^bsup>\<ge> Suc n\<^esup>"
       by simp
     ultimately show ?thesis by blast
-  qed
-
-lemma HeronConf_interp_stepwise_sporadic_cases:
-  shows "\<lbrakk> \<Gamma>, n \<turnstile> ((K sporadic \<tau>) # \<Psi>) \<triangleright> \<Phi> \<rbrakk>\<^sub>c\<^sub>o\<^sub>n\<^sub>f\<^sub>i\<^sub>g
-          = \<lbrakk> \<Gamma>, n \<turnstile> \<Psi> \<triangleright> ((K sporadic \<tau>) # \<Phi>) \<rbrakk>\<^sub>c\<^sub>o\<^sub>n\<^sub>f\<^sub>i\<^sub>g
-          \<union> \<lbrakk> ((K \<Up> n) # (K \<Down> n @ \<lfloor>\<tau>\<rfloor>) # \<Gamma>), n \<turnstile> \<Psi> \<triangleright> \<Phi> \<rbrakk>\<^sub>c\<^sub>o\<^sub>n\<^sub>f\<^sub>i\<^sub>g"
-  proof -
-    have "\<lbrakk> \<Gamma>, n \<turnstile> (K sporadic \<tau>) # \<Psi> \<triangleright> \<Phi> \<rbrakk>\<^sub>c\<^sub>o\<^sub>n\<^sub>f\<^sub>i\<^sub>g = \<lbrakk>\<lbrakk> \<Gamma> \<rbrakk>\<rbrakk>\<^sub>p\<^sub>r\<^sub>i\<^sub>m \<inter> \<lbrakk>\<lbrakk> (K sporadic \<tau>) # \<Psi> \<rbrakk>\<rbrakk>\<^sub>T\<^sub>E\<^sub>S\<^sub>L\<^bsup>\<ge> n\<^esup> \<inter> \<lbrakk>\<lbrakk> \<Phi> \<rbrakk>\<rbrakk>\<^sub>T\<^sub>E\<^sub>S\<^sub>L\<^bsup>\<ge> Suc n\<^esup>"
-      by simp
-    moreover have "\<lbrakk> \<Gamma>, n \<turnstile> \<Psi> \<triangleright> ((K sporadic \<tau>) # \<Phi>) \<rbrakk>\<^sub>c\<^sub>o\<^sub>n\<^sub>f\<^sub>i\<^sub>g = \<lbrakk>\<lbrakk> \<Gamma> \<rbrakk>\<rbrakk>\<^sub>p\<^sub>r\<^sub>i\<^sub>m \<inter> \<lbrakk>\<lbrakk> \<Psi> \<rbrakk>\<rbrakk>\<^sub>T\<^sub>E\<^sub>S\<^sub>L\<^bsup>\<ge> n\<^esup> \<inter> \<lbrakk>\<lbrakk> (K sporadic \<tau>) # \<Phi> \<rbrakk>\<rbrakk>\<^sub>T\<^sub>E\<^sub>S\<^sub>L\<^bsup>\<ge> Suc n\<^esup>"
-      by simp
-    moreover have "\<lbrakk> ((K \<Up> n) # (K \<Down> n @ \<lfloor>\<tau>\<rfloor>) # \<Gamma>), n \<turnstile> \<Psi> \<triangleright> \<Phi> \<rbrakk>\<^sub>c\<^sub>o\<^sub>n\<^sub>f\<^sub>i\<^sub>g = \<lbrakk>\<lbrakk> ((K \<Up> n) # (K \<Down> n @ \<lfloor>\<tau>\<rfloor>) # \<Gamma>) \<rbrakk>\<rbrakk>\<^sub>p\<^sub>r\<^sub>i\<^sub>m \<inter> \<lbrakk>\<lbrakk> \<Psi> \<rbrakk>\<rbrakk>\<^sub>T\<^sub>E\<^sub>S\<^sub>L\<^bsup>\<ge> n\<^esup> \<inter> \<lbrakk>\<lbrakk> \<Phi> \<rbrakk>\<rbrakk>\<^sub>T\<^sub>E\<^sub>S\<^sub>L\<^bsup>\<ge> Suc n\<^esup>"
-      by simp
-    ultimately show ?thesis
-    proof -
-      have "(\<lbrakk> K \<Up> n \<rbrakk>\<^sub>p\<^sub>r\<^sub>i\<^sub>m \<inter> \<lbrakk> K \<Down> n @ \<lfloor> \<tau> \<rfloor> \<rbrakk>\<^sub>p\<^sub>r\<^sub>i\<^sub>m \<union> \<lbrakk> K sporadic \<tau> \<rbrakk>\<^sub>T\<^sub>E\<^sub>S\<^sub>L\<^bsup>\<ge> Suc n\<^esup>) \<inter> \<lbrakk>\<lbrakk> \<Psi> \<rbrakk>\<rbrakk>\<^sub>T\<^sub>E\<^sub>S\<^sub>L\<^bsup>\<ge> n\<^esup> = \<lbrakk>\<lbrakk> (K sporadic \<tau>) # \<Psi> \<rbrakk>\<rbrakk>\<^sub>T\<^sub>E\<^sub>S\<^sub>L\<^bsup>\<ge> n\<^esup>"
-        using TESL_interp_stepwise_sporadic_coind_unfold TESL_interpretation_stepwise_cons_morph by blast
-  then have "\<lbrakk> \<Gamma>, n \<turnstile> ((K sporadic \<tau>) # \<Psi>) \<triangleright> \<Phi> \<rbrakk>\<^sub>c\<^sub>o\<^sub>n\<^sub>f\<^sub>i\<^sub>g = (\<lbrakk>\<lbrakk> ((K \<Up> n) # (K \<Down> n @ \<lfloor> \<tau> \<rfloor>) # \<Gamma>) \<rbrakk>\<rbrakk>\<^sub>p\<^sub>r\<^sub>i\<^sub>m \<inter> \<lbrakk>\<lbrakk> \<Psi> \<rbrakk>\<rbrakk>\<^sub>T\<^sub>E\<^sub>S\<^sub>L\<^bsup>\<ge> n\<^esup> \<union> \<lbrakk>\<lbrakk> \<Gamma> \<rbrakk>\<rbrakk>\<^sub>p\<^sub>r\<^sub>i\<^sub>m \<inter> \<lbrakk>\<lbrakk> \<Psi> \<rbrakk>\<rbrakk>\<^sub>T\<^sub>E\<^sub>S\<^sub>L\<^bsup>\<ge> n\<^esup> \<inter> \<lbrakk> K sporadic \<tau> \<rbrakk>\<^sub>T\<^sub>E\<^sub>S\<^sub>L\<^bsup>\<ge> Suc n\<^esup>) \<inter> \<lbrakk>\<lbrakk> \<Phi> \<rbrakk>\<rbrakk>\<^sub>T\<^sub>E\<^sub>S\<^sub>L\<^bsup>\<ge> Suc n\<^esup>"
-    by auto
-      then show ?thesis
-        by (simp add: Int_Un_distrib2 Int_assoc Un_commute)
-    qed
   qed
 
 lemma HeronConf_interp_stepwise_sporadicon_cases:
@@ -463,6 +429,12 @@ lemma HeronConf_interp_stepwise_implies_cases:
         by (simp add: Int_Un_distrib2 inf_sup_aci(2))
     qed
   qed
+
+lemma HeronConf_interp_stepwise_implies_not_cases:
+  shows "\<lbrakk> \<Gamma>, n \<turnstile> ((K\<^sub>1 implies not K\<^sub>2) # \<Psi>) \<triangleright> \<Phi> \<rbrakk>\<^sub>c\<^sub>o\<^sub>n\<^sub>f\<^sub>i\<^sub>g
+          = \<lbrakk> ((K\<^sub>1 \<not>\<Up> n) # \<Gamma>), n \<turnstile> \<Psi> \<triangleright> ((K\<^sub>1 implies not K\<^sub>2) # \<Phi>) \<rbrakk>\<^sub>c\<^sub>o\<^sub>n\<^sub>f\<^sub>i\<^sub>g
+          \<union> \<lbrakk> ((K\<^sub>1 \<Up> n) # (K\<^sub>2 \<not>\<Up> n) # \<Gamma>), n \<turnstile> \<Psi> \<triangleright> ((K\<^sub>1 implies not K\<^sub>2) # \<Phi>) \<rbrakk>\<^sub>c\<^sub>o\<^sub>n\<^sub>f\<^sub>i\<^sub>g"
+  sorry
 
 lemma HeronConf_interp_stepwise_timedelayed_cases:
   shows "\<lbrakk> \<Gamma>, n \<turnstile> ((K\<^sub>1 time-delayed by \<delta>\<tau> on K\<^sub>2 implies K\<^sub>3) # \<Psi>) \<triangleright> \<Phi> \<rbrakk>\<^sub>c\<^sub>o\<^sub>n\<^sub>f\<^sub>i\<^sub>g
