src/Denotational.thy
@@ -10,9 +10,7 @@ section \<open>Denotational interpretation for atomic TESL formulae\<close>
 (* Denotational interpretation of TESL atomic formulae *)
 fun TESL_interpretation_atomic
     :: "('\<tau>::linordered_field) TESL_atomic \<Rightarrow> '\<tau> run set" ("\<lbrakk> _ \<rbrakk>\<^sub>T\<^sub>E\<^sub>S\<^sub>L") where
-    "\<lbrakk> K sporadic \<tau> \<rbrakk>\<^sub>T\<^sub>E\<^sub>S\<^sub>L =
-        { \<rho>. \<exists>n::nat. hamlet ((Rep_run \<rho>) n K) = True \<and> time ((Rep_run \<rho>) n K) = \<tau> }"
-  | "\<lbrakk> K\<^sub>1 sporadic \<lfloor>\<tau>\<rfloor> on K\<^sub>2 \<rbrakk>\<^sub>T\<^sub>E\<^sub>S\<^sub>L =
+    "\<lbrakk> K\<^sub>1 sporadic \<lfloor>\<tau>\<rfloor> on K\<^sub>2 \<rbrakk>\<^sub>T\<^sub>E\<^sub>S\<^sub>L =
         { \<rho>. \<exists>n::nat. hamlet ((Rep_run \<rho>) n K\<^sub>1) = True \<and> time ((Rep_run \<rho>) n K\<^sub>2) = \<tau> }"
   | "\<lbrakk> K\<^sub>1 sporadic \<lfloor>\<tau>\<^sub>v\<^sub>a\<^sub>r(K\<^sub>i, n\<^sub>i) \<oplus> \<delta>\<tau>\<rfloor> on K\<^sub>2 \<rbrakk>\<^sub>T\<^sub>E\<^sub>S\<^sub>L =
         { \<rho>. \<exists>n::nat. hamlet ((Rep_run \<rho>) n K\<^sub>1) = True
@@ -23,6 +21,8 @@ fun TESL_interpretation_atomic
         { \<rho>. \<forall>n::nat. R (time ((Rep_run \<rho>) n K\<^sub>1), time ((Rep_run \<rho>) n K\<^sub>2)) }"
   | "\<lbrakk> master implies slave \<rbrakk>\<^sub>T\<^sub>E\<^sub>S\<^sub>L =
         { \<rho>. \<forall>n::nat. hamlet ((Rep_run \<rho>) n master) \<longrightarrow> hamlet ((Rep_run \<rho>) n slave) }"
+  | "\<lbrakk> master implies not slave \<rbrakk>\<^sub>T\<^sub>E\<^sub>S\<^sub>L =
+        { \<rho>. \<forall>n::nat. hamlet ((Rep_run \<rho>) n master) \<longrightarrow> \<not> hamlet ((Rep_run \<rho>) n slave) }"
   | "\<lbrakk> master time-delayed by \<delta>\<tau> on measuring implies slave \<rbrakk>\<^sub>T\<^sub>E\<^sub>S\<^sub>L =
         { \<rho>. \<forall>n. hamlet ((Rep_run \<rho>) n master) \<longrightarrow>
                  (let measured_time = time ((Rep_run \<rho>) n measuring) in
@@ -194,14 +194,6 @@ lemma NoSporadic_idem [simp]:
 
 lemma NoSporadic_setinc:
   shows "set (NoSporadic \<Phi>) \<subseteq> set \<Phi>"
-  by auto
-
-lemma SporadicOn_sugar_atom:
-  shows "\<lbrakk> K sporadic \<lfloor>\<tau>\<rfloor> on K \<rbrakk>\<^sub>T\<^sub>E\<^sub>S\<^sub>L = \<lbrakk> K sporadic \<tau> \<rbrakk>\<^sub>T\<^sub>E\<^sub>S\<^sub>L"
-  by auto
-
-lemma SporadicOn_sugar:
-  shows "\<lbrakk>\<lbrakk> (K sporadic \<lfloor>\<tau>\<rfloor> on K) # \<Phi> \<rbrakk>\<rbrakk>\<^sub>T\<^sub>E\<^sub>S\<^sub>L = \<lbrakk>\<lbrakk> (K sporadic \<tau>) # \<Phi> \<rbrakk>\<rbrakk>\<^sub>T\<^sub>E\<^sub>S\<^sub>L"
   by auto
 
 lemma Tagrel_affine_sugar:
